Uppaal_Networks/UPPAAL_Asm_AbsInt_Refine.thy
@@ -1,0 +1,36 @@
+theory UPPAAL_Asm_AbsInt_Refine
+imports                   
+  "HOL-Data_Structures.RBT_Map"
+  UPPAAL_Asm_AbsInt
+begin
+
+datatype 'a rbt_state_map = RBT_SM "(addr * 'a) rbt"
+
+definition RBT_SM :: "(addr * 'a) rbt \<Rightarrow> 'a state_map" where
+  "RBT_SM tree = SM (Lookup2.lookup tree)"
+
+code_datatype RBT_SM
+
+lemma entry_RBT_SM[code]:
+  "entry (set states) = propagate (RBT_SM empty) (set states)" sorry
+
+lemma lookup_RBT_SM[code]:
+  "lookup (RBT_SM tree) = Lookup2.lookup tree" sorry
+
+lemma domain_RBT_SM[code]:
+  "domain (RBT_SM tree) = fst ` set (inorder tree)" sorry
+
+lemma propagate_RBT_SM[code]:
+  "propagate (RBT_SM oldtree) (set ss) =
+    RBT_SM (fold (\<lambda>(pc, st) tree.
+      let newsts = (
+        case Lookup2.lookup tree pc of
+          Some sts \<Rightarrow> sts \<union> {st} |
+          None \<Rightarrow> {st})
+      in upd pc newsts tree
+    ) ss oldtree)" sorry
+
+lemma[code]: "step_all op pc (set instates) =
+  Option.these (set (map (\<lambda>ins. step op (pc, ins)) instates))" using in_these_eq by fastforce
+
+end
